BinarySearch.lean
@@ -7,5 +7,6 @@ import BinarySearch.Fake
 import BinarySearch.Interp
 import BinarySearch.IR
 import BinarySearch.Program
+import BinarySearch.ProgramCorrect
 import BinarySearch.ProgramDriver
 import BinarySearch.ProgramTest
