BinarySearch/ProgramCorrect.lean
@@ -1,0 +1,32 @@
+import BinarySearch.Basic
+import BinarySearch.Interp
+import BinarySearch.ProgramDriver
+
+set_option linter.style.header false
+
+/-! Proof that the binary search program defined in `Program.lean` when passed
+through the interpreter in `Interp.lean` produces the same result as the Lean
+implementation in `Basic.lean` -/
+
+namespace BinarySearch.ProgramCorrect
+
+open BinarySearch.Interp
+
+/-! Defines what it means for the program results to match the output of the
+native Lean search -/
+
+def resultsMatch (resultIR : Result) (ResultLean : Option Nat) : Prop :=
+  match resultIR, ResultLean with
+  | Result.return_index i, some j => i = j
+  | Result.return_none, none => True
+  | _, _ => False
+
+/-! The main theorem: the binary search IR implementation produces the same
+result as the native Lean implementation -/
+theorem binarySearch_correct (arr : Array Nat) (target low high : Nat)
+  (hhigh : high ≤ arr.size) (hsorted : Sorted arr) :
+  resultsMatch (BinarySearch.ProgramDriver.binarySearch arr target low high)
+    (binarySearch arr target low high hhigh) := by
+  sorry
+
+end BinarySearch.ProgramCorrect
